use Vocab in IsBisim
Now also the set of atomic programs can be restricted.

Pdl/Bisimulation.lean
@@ -7,73 +7,70 @@ import Pdl.Vocab
 
 section Bisim
 
-variable {W : Type} (M : KripkeModel W) (Z : W → W → Prop) (letters : ℕ → Prop)
+variable {W : Type} (M : KripkeModel W) (Z : W → W → Prop) (vo : Vocab)
 
-/-- A bisimulation on `M`, for the proposition letters in `letters`. -/
+/-- A bisimulation on `M`, for the given vocabulary. -/
 structure IsBisim : Prop where
   symm : ∀ x y, Z x y → Z y x
-  atoms : ∀ x y, Z x y → ∀ n, letters n → (M.val x n ↔ M.val y n)
-  zig : ∀ x y, Z x y → ∀ c x', M.Rel c x x' → ∃ y', M.Rel c y y' ∧ Z x' y'
+  atoms : ∀ x y, Z x y → ∀ n ∈ vo.atomProps, (M.val x n ↔ M.val y n)
+  zig : ∀ x y, Z x y → ∀ c ∈ vo.atomProgs, ∀ x', M.Rel c x x' → ∃ y', M.Rel c y y' ∧ Z x' y'
 
 variable {M Z letters}
 
 mutual
 
-theorem IsBisim.relate (hZ : IsBisim M Z letters) :
-    ∀ (α : Program) (x y x' : W), (∀ n, Sum.inl n ∈ α.voc → letters n) →
-    Z x y → relate M α x x' → ∃ y', relate M α y y' ∧ Z x' y'
-  | ·c, x, y, x', hv, hxy, h => hZ.zig x y hxy c x' h
-  | α ;' β, x, y, x', hv, hxy, h => by
+theorem IsBisim.relate (hZ : IsBisim M Z vo) :
+    ∀ α, α.voc ⊆ vo → ∀ x y x', Z x y → relate M α x x' → ∃ y', relate M α y y' ∧ Z x' y'
+  | ·c, hv, x, y, x', hxy, h => hZ.zig x y hxy c (by simp_all [Vocab.atomProgs]) x' h
+  | α ;' β, hv, x, y, x', hxy, h => by
       obtain ⟨z, h1, h2⟩ := h
-      obtain ⟨z', h1', hzz'⟩ := hZ.relate α x y z (by grind [Program.voc]) hxy h1
-      obtain ⟨y', h2', hy'⟩ := hZ.relate β z z' x' (by grind [Program.voc]) hzz' h2
+      obtain ⟨z', h1', hzz'⟩ := hZ.relate α (by simp_all; grind) x y z (by grind [Program.voc]) h1
+      obtain ⟨y', h2', hy'⟩ := hZ.relate β (by simp_all; grind) z z' x' (by grind [Program.voc]) h2
       exact ⟨y', ⟨z', h1', h2'⟩, hy'⟩
-  | α ⋓ β, x, y, x', hv, hxy, h => by
+  | α ⋓ β, hv, x, y, x', hxy, h => by
       rcases h with hα | hβ
-      · obtain ⟨y', h', hy'⟩ := hZ.relate α x y x' (by grind [Program.voc]) hxy hα
+      · obtain ⟨y', h', hy'⟩ := hZ.relate α (by simp_all; grind) x y x' (by grind [Program.voc]) hα
         exact ⟨y', Or.inl h', hy'⟩
-      · obtain ⟨y', h', hy'⟩ := hZ.relate β x y x' (by grind [Program.voc]) hxy hβ
+      · obtain ⟨y', h', hy'⟩ := hZ.relate β (by simp_all; grind) x y x' (by grind [Program.voc]) hβ
         exact ⟨y', Or.inr h', hy'⟩
-  | ∗α, x, y, x', hv, hxy, h => by
+  | ∗α, hv, x, y, x', hxy, h => by
       simp only [_root_.relate] at h ⊢
       induction h generalizing y with
       | refl => exact ⟨y, Relation.ReflTransGen.refl, hxy⟩
       | tail _ hstep IH =>
           obtain ⟨z', hz', hzz'⟩ := IH y hxy
-          obtain ⟨y', hy', hy''⟩ := hZ.relate α _ z' _ (by grind [Program.voc]) hzz' hstep
+          obtain ⟨y', hy', hy''⟩ := hZ.relate α (by simp_all) _ z' _ (by grind [Program.voc]) hstep
           exact ⟨y', Relation.ReflTransGen.tail hz' hy', hy''⟩
-  | ?'τ, x, y, x', hv, hxy, h => by
-      simp
-      simp at h
+  | ?'τ, hv, x, y, x', hxy, h => by
+      simp only [Program.voc, _root_.relate, ↓existsAndEq, true_and] at *
       rcases h with ⟨same_x, x_τ⟩
       have IH := IsBisim.evaluate hZ τ (by grind [Program.voc]) x y hxy
       rw [IH] at x_τ
       subst same_x
       exact ⟨x_τ, hxy⟩
 
-theorem IsBisim.evaluate (hZ : IsBisim M Z letters) : ∀ (φ : Formula),
-    (∀ n, Sum.inl n ∈ φ.voc → letters n) →
-    ∀ x y, Z x y → (evaluate M x φ ↔ evaluate M y φ)
+theorem IsBisim.evaluate (hZ : IsBisim M Z vo) :
+    ∀ φ, φ.voc ⊆ vo → ∀ x y, Z x y → (evaluate M x φ ↔ evaluate M y φ)
   | ⊥, _, _, _, _ => Iff.rfl
-  | ·n, hv, x, y, hxy => hZ.atoms x y hxy n (hv n (by simp))
+  | ·n, hv, x, y, hxy => hZ.atoms x y hxy n (by simp_all [Vocab.atomProps])
   | ~φ, hv, x, y, hxy => by
       simp only [_root_.evaluate]
-      rw [hZ.evaluate φ (fun n hn => hv n (by simpa using hn)) x y hxy]
+      rw [hZ.evaluate φ (fun n hn => by simp_all; grind) x y hxy]
   | φ ⋀ ψ, hv, x, y, hxy => by
       simp only [_root_.evaluate]
-      rw [hZ.evaluate φ (fun n hn => hv n (by simp [hn])) x y hxy,
-        hZ.evaluate ψ (fun n hn => hv n (by simp [hn])) x y hxy]
+      rw [hZ.evaluate φ (fun n hn => by simp_all; grind) x y hxy,
+        hZ.evaluate ψ (fun n hn => by simp_all; grind) x y hxy]
   | ⌈α⌉ φ, hv, x, y, hxy => by
-      have hvφ : ∀ n, Sum.inl n ∈ φ.voc → letters n := fun n hn => hv n (by simp [hn])
+      have hvφ : φ.voc ⊆ vo := fun n hn => by simp_all; grind
       simp only [_root_.evaluate]
       constructor
       · intro h y' hyy'
         obtain ⟨x', hxx', hx'y'⟩ :=
-          hZ.relate α y x y' (by grind [Formula.voc]) (hZ.symm x y hxy) hyy'
+          hZ.relate α (by simp_all; grind) y x y' (hZ.symm x y hxy) hyy'
         exact (hZ.evaluate φ hvφ x' y' (hZ.symm _ _ hx'y')).mp (h x' hxx')
       · intro h x' hxx'
         obtain ⟨y', hyy', hx'y'⟩ :=
-          hZ.relate α x y x' (by grind [Formula.voc]) hxy hxx'
+          hZ.relate α (by simp_all; grind) x y x' (by simp_all) hxx'
         exact (hZ.evaluate φ hvφ x' y' hx'y').mpr (h y' hyy')
 
 end -- mutual
